More updates; Add Pset6

lectures/Lowstar/code/RevSeq.fst
@@ -25,5 +25,32 @@ let rec rev_seq' s i =
 
 let rev_seq s = rev_seq' s 0
 
+val rev_lemma_step : #a:eqtype -> orig:seq a -> cur:seq a -> i:nat ->
+  Pure (seq a) (requires
+          (let l = Seq.length orig in
+            (Seq.length cur = l) /\
+            (i < l/2) /\
+            (seq_to_list (Seq.slice cur 0 i) = rev_list (seq_to_list (Seq.slice orig (l - i - 1) l))) /\
+            (seq_to_list (Seq.slice cur (l - i - 1) l) = rev_list (seq_to_list (Seq.slice orig 0 i))) /\
+            (seq_to_list (Seq.slice cur i (l - i)) = seq_to_list (Seq.slice orig i (l - i)))))
+        (ensures
+          (fun cur ->
+            let l = Seq.length orig in
+            (Seq.length cur = l) /\
+            (seq_to_list (Seq.slice cur 0 (i+1)) = rev_list (seq_to_list (Seq.slice orig (l - i - 2) l))) /\
+            (seq_to_list (Seq.slice cur (l - i - 2) l) = rev_list (seq_to_list (Seq.slice orig 0 (i+1)))) /\
+            (seq_to_list (Seq.slice cur (i+1) (l - i - 1)) = seq_to_list (Seq.slice orig (i+1) (l - i - 1)))))
+let rev_lemma_step orig cur i =
+  let ei = Seq.index cur i in
+  let ei' = Seq.index cur (Seq.length cur - i - 1) in
+  let cur' = Seq.upd cur i ei' in
+  let cur'' = Seq.upd cur' (Seq.length cur - i - 1) ei in
+  let res = cur'' in
+  let l = Seq.length orig in
+  assert (Seq.length cur'' = l);
+  cur''
+
+
+
 val rev_lemma : #a:eqtype -> s:seq a -> Tot (rev_list (seq_to_list s) = seq_to_list (rev_seq s))
 let rev_lemma s = admit ()
