lectures/Lowstar/code/Math.fst
@@ -1,0 +1,41 @@
+module Math
+
+open FStar.HyperStack.ST
+
+let square (x: UInt32.t): UInt32.t =
+  let open FStar.UInt32 in
+  x *%^ x
+
+let abs (x: Int32.t): Pure Int32.t
+  (requires Int32.v x <> Int.min_int 32)
+  (ensures fun r -> Int32.v r >= 0)
+=
+  let open FStar.Int32 in
+  if x >=^ 0l then
+    x
+  else
+    0l -^ x
+
+let abs2 (x: Int32.t): option Int32.t =
+  let open FStar.Int32 in
+  if Int32.v x = Int.min_int 32 then
+    None
+  else if x >=^ 0l then
+    Some x
+  else
+    Some (0l -^ x)
+
+(* Algebraic data types are compiled to tagged enums 
+
+typedef enum { FStar_Pervasives_Native_None, FStar_Pervasives_Native_Some }
+FStar_Pervasives_Native_option__int32_t_tags;
+
+typedef struct FStar_Pervasives_Native_option__int32_t_s
+{
+  FStar_Pervasives_Native_option__int32_t_tags tag;
+  int32_t v;
+}
+FStar_Pervasives_Native_option__int32_t;
+*)
+
+let main () : St Int32.t = 0l
