Notes.md
@@ -1,0 +1,3 @@
+# Notes
+
+* Pulse: https://iris-project.org/workshop-2024/slides/martinez.pdf
